simplified example

trunk/examples/termination/memSafeFail/moreSimplifiedDifficultChar.bpl
@@ -1,30 +1,21 @@
 //
-implementation cstrcpy(#in~s1 : $Pointer$, #in~s2 : $Pointer$) returns ()
+implementation cstrcpy(#ins : int, #int : int) returns ()
 {
-    var ~s1 : $Pointer$;
-    var ~s2 : $Pointer$;
-    var #t~mem1 : int;
-    var #t~mem2 : int;
-    var #t~post3 : $Pointer$;
+    var s : int;
+    var t : int;
 
-    ~s1 := #in~s1;
-    ~s2 := #in~s2;
+    s := #ins;
+    t := #int;
     while (true)
     {
-      Loop~0:
-        call #t~mem1 := read~int(~s2, 1);
-        call write~int(#t~mem1, ~s1, 1);
-        havoc #t~mem1;
-        call #t~mem2 := read~int(~s1, 1);
-        if (#t~mem2 == 0) {
-            havoc #t~mem2;
+	    assert 1 + t  <= ourLength;
+		assert 1 + s  <= ourLength;
+		memory[s] := memory[t];
+
+        if (memory[s] == 0) {
             break;
-        } else {
-            havoc #t~mem2;
-        }
-        #t~post3 := ~s2;
-        ~s2 := { base: #t~post3!base, offset: #t~post3!offset + 1 };
-        havoc #t~post3;
+        } 
+        t := t + 1 ;
     }
 }
 
@@ -33,40 +24,27 @@ implementation cstrcpy(#in~s1 : $Pointer$, #in~s2 : $Pointer$) returns ()
 implementation ULTIMATE.start() returns ()
 {
     var length : int;
-    var string : $Pointer$;
+    var string : int;
 
-    assume (length >=1);
-	assume ourLength == length;
-	assume string!offset == 0;
-	assume #memory_int[{ base: string!base, offset: string!offset + (length - 1) * 1 }] == 0;
+    assume (length >=0);
+	assume ourLength == length + 1;
+	assume string == 0;
+	assume memory[string + length] == 0;
     call cstrcpy(string, string);
 }
 
-type $Pointer$ = { base : int, offset : int };
-var #memory_int : [$Pointer$]int;
-procedure write~int(#value : int, #ptr : $Pointer$, #sizeOfWrittenType : int) returns ();
-//    requires #valid[#ptr!base];
-//    requires #sizeOfWrittenType + #ptr!offset <= #length[#ptr!base];
-    modifies #memory_int;
-    ensures #memory_int == old(#memory_int)[#ptr := #value];
+var memory : [int]int;
 
-procedure read~int(#ptr : $Pointer$, #sizeOfReadType : int) returns (#value : int);
-//    requires #valid[#ptr!base];
-    requires #sizeOfReadType + #ptr!offset <= ourLength;
-    ensures #value == #memory_int[#ptr];
-
-var #valid : [int]bool;
-var #length : [int]int;
 var ourLength : int;
 
 procedure __VERIFIER_nondet_int() returns (#res : int);
     modifies ;
 
-procedure cstrcpy(#in~s1 : $Pointer$, #in~s2 : $Pointer$) returns ();
-    modifies #memory_int;
+procedure cstrcpy(#ins : int, #int : int) returns ();
+    modifies memory;
 
 
 procedure ULTIMATE.start() returns ();
-    modifies #valid, #memory_int;
-    modifies #memory_int, #valid, #length;
+    modifies memory;
+    modifies memory;
 
